nola/iris/cif.v
@@ -1,0 +1,183 @@
+(** * [cif]: Coinductive-inductive set of formulas *)
+
+From nola.util Require Export fn cit.
+From nola.bi Require Import ofe.
+From nola.iris Require Export ofe.
+Import iPropAppNotation.
+
+(** ** Data types *)
+
+(** [cif_binsel]: Binary operator selector *)
+Variant cif_binsel :=
+| (** Conjunction *) cifs_and
+| (** Disjunction *) cifs_or
+| (** Implication *) cifs_imp
+| (** Separating conjunction *) cifs_sep
+| (** Magic wand *) cifs_wand.
+
+(** [cif_unsel]: Unary operator selector *)
+Variant cif_unsel :=
+| (** Plainly *) cifs_plain
+| (** Persistently *) cifs_pers
+| (** Basic update *) cifs_bupd
+| (** Except-0 *) cifs_except0.
+
+(** [cif_sel]: Selector *)
+Variant cif_sel S :=
+| (** Universal quantifier *) cifs_all (A : Type)
+| (** Existential quantifier *) cifs_ex (A : Type)
+| (** Binary operator *) cifs_bin (s : cif_binsel)
+| (** Unary operator *) cifs_un (s : cif_unsel)
+| (** Pure proposition *) cifs_pure
+| (** Later *) cifs_later
+| (** Custom selector *) cifs_custom (s : S).
+Arguments cifs_all {_}. Arguments cifs_ex {_}.
+Arguments cifs_bin {_}.  Arguments cifs_un {_}.
+Arguments cifs_pure {_}. Arguments cifs_later {_}. Arguments cifs_custom {_}.
+
+(** [cif_idom]: Domain for inductive parts *)
+Definition cif_idom {S} (I : S → Type) (s : cif_sel S) : Type := match s with
+  | cifs_all A | cifs_ex A => A | cifs_bin _ => bool | cifs_un _ => unit
+  | cifs_pure | cifs_later => Empty_set | cifs_custom s => I s
+  end.
+
+(** [cif_cdom]: Domain for coinductive parts *)
+Definition cif_cdom {S} (C : S → Type) (s : cif_sel S) : Type := match s with
+  | cifs_all _ | cifs_ex _ | cifs_bin _ | cifs_un _ | cifs_pure | cifs_later =>
+      Empty_set
+  | cifs_custom s => C s
+  end.
+
+(** [cif_dataOF]: Data [oFunctor] *)
+Definition cif_dataOF {S} (D : S → oFunctor) (s : cif_sel S) : oFunctor :=
+  match s with
+  | cifs_all _ | cifs_ex _ | cifs_bin _ | cifs_un _ => unitO
+  | cifs_pure => PropO | cifs_later => laterOF ∙ | cifs_custom s => D s
+  end.
+
+(** [cif_dataOF] is contractive *)
+#[export] Instance cif_dataOF_contractive {S s}
+  `{∀ s : S, oFunctorContractive (D s)} : oFunctorContractive (cif_dataOF D s).
+Proof. case s=>/=; exact _. Qed.
+
+(** ** [cif]: Coinductive-inductive set of formulas *)
+Definition cifOF {S} I C D : oFunctor :=
+  citOF (cif_idom (S:=S) I) (cif_cdom C) (cif_dataOF D).
+Definition cif {S} I C D Σ : Type := cifOF (S:=S) I C D $oi Σ.
+
+(** [cifOF] is contractive *)
+Fact cifOF_contractive {S I C} `{∀ s, oFunctorContractive (D s)} :
+  oFunctorContractive (@cifOF S I C D).
+Proof. exact _. Qed.
+
+(** ** Construct [cif] *)
+Section cif.
+  Context {S} {I C : S → Type} {D : S → oFunctor} {Σ : gFunctors}.
+  Implicit Type Px Qx : cif I C D Σ.
+
+  Definition cif_all {A} (Φxs : A -d> cif I C D Σ) : cif I C D Σ :=
+    CitX (cifs_all A) Φxs nullary ().
+  Definition cif_ex {A} (Φxs : A -d> cif I C D Σ) : cif I C D Σ :=
+    CitX (cifs_ex A) Φxs nullary ().
+
+  Definition cif_bin s Px Qx : cif I C D Σ :=
+    CitX (cifs_bin s) (binary Px Qx) nullary ().
+  Definition cif_and := cif_bin cifs_and.
+  Definition cif_or := cif_bin cifs_or.
+  Definition cif_imp := cif_bin cifs_imp.
+  Definition cif_sep := cif_bin cifs_sep.
+  Definition cif_wand := cif_bin cifs_wand.
+
+  Definition cif_un s Px : cif I C D Σ :=
+    CitX (cifs_un s) (unary Px) nullary ().
+  Definition cif_plain := cif_un cifs_plain.
+  Definition cif_pers := cif_un cifs_pers.
+  Definition cif_bupd := cif_un cifs_bupd.
+  Definition cif_except0 := cif_un cifs_except0.
+
+  Definition cif_pure (φ : Prop) : cif I C D Σ :=
+    CitX cifs_pure nullary nullary φ.
+  Definition cif_later (P : iProp Σ) : cif I C D Σ :=
+    CitX cifs_later nullary nullary (Next P%I).
+
+  Definition cif_custom s (Φxs : I s -d> cif I C D Σ)
+    (Ψxs : C s -d> cif I C D Σ) (d : D s $oi Σ) : cif I C D Σ :=
+    CitX (cifs_custom s) Φxs Ψxs d.
+
+  (** Non-expansiveness *)
+  #[export] Instance cif_all_ne {A} : NonExpansive (@cif_all A).
+  Proof. move=> ????. apply Cit_ne, CitI_ne; solve_proper. Qed.
+  #[export] Instance cif_ex_ne {A} : NonExpansive (@cif_ex A).
+  Proof. move=> ????. apply Cit_ne, CitI_ne; solve_proper. Qed.
+  #[export] Instance cif_bin_ne {s} : NonExpansive2 (cif_bin s).
+  Proof. move=> ???????. apply Cit_ne, CitI_ne; solve_proper. Qed.
+  #[export] Instance cif_un_ne {s} : NonExpansive (cif_un s).
+  Proof. move=> ????. apply Cit_ne, CitI_ne; solve_proper. Qed.
+  #[export] Instance cif_pure_ne : NonExpansive cif_pure.
+  Proof. move=> ????. apply Cit_ne, CitI_ne; solve_proper. Qed.
+  #[export] Instance cif_later_ne : NonExpansive cif_later.
+  Proof. move=> ????. apply Cit_ne, CitI_ne; solve_proper. Qed.
+  #[export] Instance cif_custom_ne {s} : NonExpansive3 (cif_custom s).
+  Proof. move=> ??????????. apply Cit_ne, CitI_ne; solve_proper. Qed.
+End cif.
+
+Declare Scope cif_scope.
+Delimit Scope cif_scope with n.
+Bind Scope cif_scope with cif.
+Notation "∀ x .. y , Px" :=
+  (cif_all (λ x, .. (cif_all (λ y, Px%n)) ..)) : cif_scope.
+Notation "∃ x .. y , Px" :=
+  (cif_ex (λ x, .. (cif_ex (λ y, Px%n)) ..)) : cif_scope.
+Infix "→" := cif_imp : cif_scope.
+Infix "∗" := cif_sep : cif_scope.
+Infix "-∗" := cif_wand : cif_scope.
+Notation "■ Px" := (cif_plain Px) : cif_scope.
+Notation "□ Px" := (cif_pers Px) : cif_scope.
+Notation "|==> Px" := (cif_bupd Px) : cif_scope.
+Notation "◇ Px" := (cif_except0 Px) : cif_scope.
+Notation "⌜ φ ⌝" := (cif_pure φ) : cif_scope.
+Notation "'True'" := (cif_pure True) : cif_scope.
+Notation "'False'" := (cif_pure False) : cif_scope.
+Notation "▷ P" := (cif_later P) : cif_scope.
+
+(** ** [cif_intp]: Interpretation of [cif] *)
+Section iris.
+  Context {S} {I C : S → Type} {D : S → oFunctor} {Σ : gFunctors}.
+
+  (** [cif_bintp]: Base interpretation for [cif] *)
+  Definition cif_bintp
+    (ip : ∀ s, (I s -d> iProp Σ) → (C s -d> cif I C D Σ) →
+      D s $oi Σ → iProp Σ) s
+    : (cif_idom I s -d> iProp Σ) → (cif_cdom C s -d> cif I C D Σ) →
+        cif_dataOF D s $oi Σ → iProp Σ :=
+    match s with
+    | cifs_all _ => λ Ps _ _, ∀ a, Ps a | cifs_ex _ => λ Ps _ _, ∃ a, Ps a
+    | cifs_bin s => λ Ps _ _, let P := Ps true in let Q := Ps false in
+        match s with
+        | cifs_and => P ∧ Q | cifs_or => P ∨ Q | cifs_imp => P → Q
+        | cifs_sep => P ∗ Q | cifs_wand => P -∗ Q
+        end
+    | cifs_un s => λ Ps _ _, let P := Ps () in
+        match s with
+        | cifs_plain => ■ P | cifs_pers => □ P | cifs_bupd => |==> P
+        | cifs_except0 => ◇ P
+        end
+    | cifs_pure => λ _ _ φ, ⌜φ⌝ | cifs_later => λ _ _, laterl
+    | cifs_custom s => ip s
+    end%I.
+
+  (** [cif_bintp] is non-expansive *)
+  #[export] Instance cif_bintp_ne `{!∀ s, NonExpansive3 (ip s)} {s} :
+    NonExpansive3 (cif_bintp ip s).
+  Proof.
+    case s=>/=; try solve_proper. move=> ???????. by apply laterl_ne.
+  Qed.
+
+  (** [cif_intp]: Interpretation of [cif] *)
+  Definition cif_intp ip : cif I C D Σ → iProp Σ := cit_intp (cif_bintp ip).
+
+  (** [cif_intp ip] is non-expansive if [ip] is *)
+  Fact cif_intp_ne `{!∀ s, NonExpansive3 (ip s)} : NonExpansive (cif_intp ip).
+  Proof. exact _. Qed.
+End iris.
+Arguments cif_intp {_ _ _ _ _} _ _ /.
